Add (fdom,fapply,flookup,fupdate) lemmas for projectS

projection/bakery_to_endpointScript.sml
@@ -46,11 +46,50 @@ val project_def = Define `
    state `var |-> val`
 *)
 val projectS_def = Define`
-  projectS p s =
-    let state_of_p = FILTER (λx. SND (FST x) = p) (fmap_to_alist s);
-        v_to_vl    = MAP (λx. (FST (FST x), SND x)) state_of_p;
-    in alist_to_fmap v_to_vl
+  projectS p s = MAP_KEYS (λx. FST x) (DRESTRICT s (λx. SND x = p))
 `;
+
+(* The domain of a state `s` projected to a process `p` is the set of
+   all variable names associated with `p` in the domain of `s`
+*)
+val fdom_projectS = Q.store_thm("fdom_projectS",
+  `∀p s. FDOM (projectS p s) = { v | (v,p) ∈ FDOM s }`,
+  rw [projectS_def,MAP_KEYS_def,DRESTRICT_DEF,IMAGE_DEF,FUN_EQ_THM]
+  \\ EQ_TAC >> rw [] >> fs [] >> Q.EXISTS_TAC `(x,p)` >> rw [] );
+
+
+(* If a key `(v,p)` is in the domain of a global state `s` then
+   one can expect the application of the projected key `v` over
+   a projected state `projectS p s` to be equal to an original
+   (un-projected) application
+*)
+val fapply_projectS = Q.store_thm("fapply_projectS",
+  `∀p v (s : β # α |-> γ). (v,p) ∈ FDOM s ⇒ projectS p s ' v = s ' (v,p)`,
+  rw [projectS_def,MAP_KEYS_def,DRESTRICT_DEF]
+  \\ sg `INJ FST (FDOM (DRESTRICT s (λx. SND x = p))) 𝕌(:β)`
+  >- rw [DRESTRICT_DEF,INJ_DEF,PAIR_FST_SND_EQ]
+  \\ IMP_RES_TAC (MAP_KEYS_def |> CONV_RULE (TOP_DEPTH_CONV FORALL_AND_CONV) |> CONJUNCT2)
+  \\ first_x_assum (ASSUME_TAC o Q.SPEC `(v,p)`)
+  \\ rfs [DRESTRICT_DEF,ETA_THM]
+);
+
+(* If a value is available on a state `s` with key `(v,p)` then it
+   should also be available in a projected state `projectS p s` with
+   key `v`
+*)
+val lookup_projectS = Q.store_thm("lookup_projectS",
+  `∀p v s d. FLOOKUP s (v,p) = SOME d ⇒ FLOOKUP (projectS p s) v = SOME d`,
+  rw [FLOOKUP_DEF,fapply_projectS,fdom_projectS]
+);
+
+(* If a state is updated with bindings for a process (`p2`) this does not
+   affect the projection of any other process (`p1`)
+*)
+val fupdate_projectS = Q.store_thm("fupdate_projectS",
+  `∀p1 p2 s v d. p1 ≠ p2 ⇒ projectS p1 (s |+ ((v,p2),d)) = projectS p1 s`,
+  rw [projectS_def]
+);
+
 
 (*Crates a network of projections from a choreography *)
 val compile_network_def = Define`
